Make the first step of splitter refinement faster

src/Parsers/Refinement/IndexedAndAtMostOneNonTerminalReflectiveOpt.v
@@ -431,7 +431,7 @@ Section IndexedImpl_opt.
   Local Arguments opt.leb !_ !_.
   Local Arguments opt.minus !_ !_.
 
-  Definition FirstStep_sig
+  Definition FirstStep0_sig
   : { sp : _ & refineADT (string_spec G HSL) sp }.
   Proof.
     eexists.
@@ -571,8 +571,63 @@ Section IndexedImpl_opt.
     apply reflexivityT.
   Defined.
 
+  Definition opt_rindexed_spec0
+    := Eval cbv [projT1 FirstStep0_sig] in projT1 FirstStep0_sig.
+
+  Lemma FirstStep0
+    : refineADT (string_spec G HSL) opt_rindexed_spec0.
+  Proof.
+    apply (projT2 FirstStep0_sig).
+  Qed.
+
+  Definition opt_rindexed_spec_method_default : String -> nat * (nat * nat) -> nat -> nat -> Comp (String * list nat).
+  Proof.
+    let c := (eval cbv [opt_rindexed_spec0] in opt_rindexed_spec0) in
+    let c := lazymatch c with
+             | appcontext[fun r_n d d0 d1 => Bind (opt2.fold_right (@?f r_n d d0 d1) ?init ?ls) (fun a => @?retv r_n d d0 d1 a)]
+               => (eval cbv beta in (fun r_n d d0 d1 => Bind (opt2.fold_right (f r_n d d0 d1) init ls) (fun a => retv r_n d d0 d1 a)))
+             end in
+    exact c.
+  Defined.
+
+  Section gen.
+    Context c
+            (Href : forall str d d0 d1, refine (opt_rindexed_spec_method_default str d d0 d1) (c str d d0 d1)).
+
+    Definition FirstStep_sig_gen
+      : { sp : _ & refineADT (string_spec G HSL) sp }.
+    Proof.
+      eexists.
+      eapply transitivityT; [ apply FirstStep0 | ].
+      unfold opt_rindexed_spec0.
+      hone method "splits".
+      {
+        setoid_rewrite refineEquiv_pick_eq'.
+        simplify with monad laws.
+        simpl; subst_body; subst.
+        cbv [opt_rindexed_spec_method_default] in Href.
+        apply Href.
+      }
+      cbv beta.
+      apply reflexivityT.
+    Defined.
+
+    Definition opt_rindexed_spec_gen
+      := Eval cbv [projT1 FirstStep_sig_gen] in projT1 FirstStep_sig_gen.
+
+    Lemma FirstStep_gen
+      : refineADT (string_spec G HSL) opt_rindexed_spec_gen.
+    Proof.
+      apply (projT2 FirstStep_sig_gen).
+    Qed.
+  End gen.
+
+  Definition FirstStep_sig
+    : { sp : _ & refineADT (string_spec G HSL) sp }
+    := FirstStep_sig_gen _ (fun _ _ _ _ => reflexivity _).
+
   Definition opt_rindexed_spec
-    := Eval cbv [projT1 FirstStep_sig] in projT1 FirstStep_sig.
+    := Eval cbv [projT1 FirstStep_sig FirstStep_sig_gen opt_rindexed_spec_method_default] in projT1 FirstStep_sig.
 
   Lemma FirstStep
     : refineADT (string_spec G HSL) opt_rindexed_spec.
@@ -641,4 +696,119 @@ Section tower.
     intros.
     setoid_rewrite_hyp; reflexivity.
   Qed.
+
+  Fixpoint make_tower_no_unif base (ls : list A) new_comp concl
+    := match ls with
+       | nil => refine (x0 <- new_comp base; r_o x0) retv
+                -> concl
+       | cons x xs
+         => match proj x with
+            | ret_pick _
+              => forall part_retv,
+                (test x -> refine (test_true x) part_retv)
+                -> make_tower_no_unif
+                     base
+                     xs
+                     (fun new_comp' => new_comp (If test x Then part_retv Else new_comp'))
+                     concl
+            | _
+              => make_tower_no_unif
+                   base
+                   xs
+                   (fun new_comp' => new_comp (If test x Then test_true x Else new_comp'))
+                   concl
+            end
+       end.
+
+  Lemma make_tower_const base ls v v'
+        (H : refine v' v)
+    : make_tower base ls (fun _ => v) (fun _ => v').
+  Proof.
+    induction ls as [|x xs IHxs]; simpl.
+    { rewrite H; intro; assumption. }
+    { destruct (proj x); intros; assumption. }
+  Qed.
+
+  Lemma make_tower_no_unif_const base ls v v'
+        (H : refine v' v)
+    : make_tower_no_unif base ls (fun _ => v) (refine (x0 <- v'; r_o x0) retv).
+  Proof.
+    induction ls as [|x xs IHxs]; simpl.
+    { rewrite H; intro; assumption. }
+    { destruct (proj x); intros; assumption. }
+  Qed.
+
+  Lemma refine_opt2_fold_right_no_unif base ls
+    : make_tower_no_unif base ls (fun x => x) (refine (x0 <- opt2.fold_right (fun x else_case => If test x Then test_true x Else else_case) base ls; r_o x0) retv).
+  Proof.
+    pose proof (refine_opt2_fold_right base ls) as H.
+    induction ls as [|x xs IHxs].
+    { exact H. }
+    { simpl in *.
+      repeat match goal with
+             | _ => assumption
+             | [ |- appcontext[If test ?x Then _ Else _] ] => destruct (test x) eqn:?
+             | _ => progress simpl in *
+             | [ |- appcontext[match ?e with _ => _ end] ] => destruct e eqn:?
+             | _ => apply make_tower_const; reflexivity
+             | _ => apply make_tower_no_unif_const; first [ reflexivity | assumption ]
+             | _ => progress intros
+             | _ => progress specialize_by ltac:(exact eq_refl)
+             | _ => progress specialize_by assumption
+             | _ => solve [ eauto with nocore ]
+             end. }
+  Qed.
 End tower.
+
+Section step_tower.
+  Context {G' : pregrammar' Ascii.ascii}
+          {HSLM : StringLikeMin Ascii.ascii}
+          {HSL : StringLike Ascii.ascii}
+          {HSLP : StringLikeProperties Ascii.ascii}
+          {HSEP : StringEqProperties Ascii.ascii}.
+  Let A := (nat * (nat * nat) * ret_cases)%type.
+  Let B := (@StringLike.String Ascii.ascii HSLM * list nat)%type.
+  Let proj : A -> ret_cases := @opt0.snd _ _.
+  Let pre_r_o : String -> list nat -> Comp B
+    := fun str => (fun x0 : list nat => ret (str, x0)).
+  Context (pre_retv : String -> nat * (nat * nat) -> nat -> nat -> Comp (String * list nat)).
+  Let test_test_true : String -> nat * (nat * nat) -> nat -> nat
+                       -> (A -> bool) * (A -> Comp (list nat)).
+  Proof.
+    intros r_o d d0 d1.
+    lazymatch (eval cbv [opt_rindexed_spec_method_default] in (opt_rindexed_spec_method_default G' r_o d d0 d1)) with
+    | appcontext[opt2.fold_right
+                   (fun a a0 => If @?test a Then @?test_true a Else a0)
+                   ?base
+                   ?ls]
+      => exact (test, test_true)
+    end.
+  Defined.
+  Let pre_test : String -> nat * (nat * nat) -> nat -> nat -> A -> bool
+    := fun r_o d d0 d1 => let '(test, test_true) := test_test_true r_o d d0 d1 in test.
+  Let pre_test_true : String -> nat * (nat * nat) -> nat -> nat -> A -> Comp (list nat)
+    := fun r_o d d0 d1 => let '(test, test_true) := test_test_true r_o d d0 d1 in test_true.
+
+  Lemma FirstStep_splits
+        (H : forall r_o d d0 d1,
+            refine (x0 <- opt2.fold_right (fun x else_case => If pre_test r_o d d0 d1 x Then pre_test_true r_o d d0 d1 x Else else_case) (ret nil) (opt.expanded_fallback_list_body G'); ret (r_o, x0)) (pre_retv r_o d d0 d1))
+        res
+        (Hres : refineADT (opt_rindexed_spec_gen pre_retv) (ComputationalADT.LiftcADT res))
+    : FullySharpened (@string_spec G' G' eq_refl HSLM HSL).
+  Proof.
+    eexists.
+    eapply transitivityT; [ | exact Hres ].
+    eapply transitivityT; [ apply (@FirstStep _ _ _ _) | ].
+    cbv [opt_rindexed_spec opt_rindexed_spec_gen].
+    hone method "splits".
+    2:apply reflexivityT.
+    {
+      setoid_rewrite General.refineEquiv_pick_eq'.
+      simplify with monad laws.
+      simpl; subst_body; subst.
+      move H at bottom.
+      cbv beta in H.
+      apply H.
+    }
+  Defined.
+End step_tower.
