src/Parsers/Refinement/Tactics.v
@@ -116,6 +116,23 @@ Proof.
   rewrite <- surjective_pairing; reflexivity.
 Qed.
 
+Ltac apply_splitter_tower_lemma :=
+  let lem := fresh in
+  change @fst with @opt0.fst;
+  change @snd with @opt0.snd;
+  lazymatch goal with
+  | [ |- refine (x0 <- (opt2.fold_right
+                          (fun a a0 => If @?test a Then @?test_true a Else a0)
+                          ?base
+                          ?ls);
+                 (@?r_o x0))
+                ?retv ]
+    => pose proof (@refine_opt2_fold_right_no_unif _ _ (@opt0.snd _ _) r_o retv test test_true base ls) as lem
+  end;
+  cbv [make_tower_no_unif opt0.snd opt0.fst] in lem |- *;
+  eapply lem; clear lem;
+  intros.
+
 Ltac simplify_parser_splitter' :=
   first [ idtac;
           match goal with
@@ -123,21 +140,7 @@ Ltac simplify_parser_splitter' :=
                         ?v ]
             => apply (@simplify_monad_laws_first_step _ _ _ c f v)
           end;
-          let lem := fresh in
-          change @fst with @opt0.fst;
-          change @snd with @opt0.snd;
-          lazymatch goal with
-          | [ |- refine (x0 <- (opt2.fold_right
-                                  (fun a a0 => If @?test a Then @?test_true a Else a0)
-                                  ?base
-                                  ?ls);
-                         (@?r_o x0))
-                        ?retv ]
-            => pose proof (@refine_opt2_fold_right _ _ (@opt0.snd _ _) r_o retv test test_true base ls) as lem
-          end;
-          cbv [make_tower opt0.snd opt0.fst] in lem |- *;
-          eapply lem; clear lem;
-          intros
+          apply_splitter_tower_lemma
         | progress autounfold with parser_sharpen_db;
           cbv beta iota zeta;
           simpl @Operations.List.uniquize;
@@ -180,11 +183,31 @@ Tactic Notation "simplify" "parser" "splitter" :=
   repeat simplify_parser_splitter'.
 
 Ltac splitter_start :=
-  start sharpening ADT;
+  let lem := match goal with
+             | [ |- FullySharpened (@string_spec _ ?G _ ?HSLM ?HSL) ]
+               => constr:(@FirstStep_splits G HSLM HSL)
+             end in
+  let lem := constr:(lem _ _) in
+  eapply lem; [ intros ???? | cbv [opt_rindexed_spec_gen] ];
+  [ let ev := match goal with
+              | [ |- refine ?x ?y ]
+                => head y
+              end in
+    is_evar ev;
+    let e := fresh in
+    set (e := ev);
+    lazymatch goal with
+    | [ |- context[opt2.fold_right _ _ ?ls] ]
+      => replace_with_vm_compute ls
+    end;
+    apply_splitter_tower_lemma
+  | ];
+  instantiate; cbv beta.
+(*start sharpening ADT;
   start honing parser using indexed representation;
   hone method "splits";
   [ simplify parser splitter
-  | ].
+  | ].*)
 
 Ltac splitter_finish :=
   idtac;
